Separation btw lambda calculus definition+ functions (Lambda_... file)  and proofs of types safety, canonical forms, ... (Ext_Structures file) TODO add typing, eval with fixpoint rules 	complete inversion, weakening lemma

2016/Ext_Structures.thy
@@ -3,6 +3,7 @@ theory Ext_Structures
 imports
    Main
    List_extra
+   Lambda_calculus
   "~~/src/HOL/List"
   "~~/src/HOL/Eisbach/Eisbach"
   "~~/src/HOL/Eisbach/Eisbach_Tools"
@@ -10,255 +11,11 @@ imports
 begin
 (*>*)
 
-section{*Pair, Tuples and Records*
+section{*Pair, Tuples and Records*}
 
 text{* In this section,we extend our current lambda calculus with extended structures (pairs, tuples, records)*}
 
-datatype ltype =
-  Nat  |
-  Bool |
-  T (num:nat) |
-  Unit |
-  Prod ltype ltype (infix "|\<times>|" 225)|
-  Fun (domain: ltype) (codomain: ltype) (infixr "\<rightarrow>" 225)|
-  TupleT "ltype list" ( "\<lparr>_\<rparr>" [150]225) |
-  RecordT "string list" "ltype list" ( "\<lparr>_|:|_\<rparr>" [150,150] 225) |
-  Sum ltype ltype (infix "|+|" 225) |
-  TVariant "string list" "ltype list" ( "<_|,|_>" [150,150] 225)
 
-datatype Lpattern = V nat | RCD "string list" "Lpattern list"
-
-datatype lterm =
-  LTrue |
-  LFalse |
-  LIf (bool_expr: lterm) (then_expr: lterm) (else_expr: lterm) |
-  LVar nat |
-  LNat nat |
-  LPlus lterm lterm |
-  LAbs (arg_type: ltype) (body: lterm) |
-  LApp lterm lterm |
-  unit |
-  Seq (fp: lterm) (sp: lterm) ("(_;;_)" [100,50] 200) |
-  AS lterm ltype ("_/ as/ _" [100,150] 200) |
-  LetBinder nat lterm lterm ("Let/ var/ (_)/ :=/ (_)/ in/ (_)" [100,120,150] 250) | 
-  Pair lterm lterm ("\<lbrace>_,_\<rbrace>" [100,150] 250) |
-  Proj1 lterm ("\<pi>1/ _" [100] 250) |
-  Proj2 lterm ("\<pi>2/ _" [100] 250) |
-  Tuple "lterm list" |
-  ProjT nat lterm ("\<Pi>/ _/ (_)" [100,150] 250) |
-  Record "string list" "lterm list" |
-  ProjR string lterm |
-  Pattern Lpattern ("<|_|>" [100] 250) |
-  LetP Lpattern lterm lterm ("Let/ pattern/ (_)/ :=/ (_)/ in/ (_)"[100,120,150]250) |
-  inl lterm ltype ("inl/ (_)/ as/ (_)" [100,100]200) |
-  inr lterm ltype ("inr/ (_)/ as/ (_)" [100,100]200) |
-  CaseSum lterm nat lterm nat lterm ("Case/ (_)/ of/ Inl/ (_)/ \<Rightarrow>/ (_)/ |/ Inr/ (_)/ \<Rightarrow>/ (_)" [100, 100,100, 100, 100]200) |
-  Variant string lterm ltype ("<(_):=(_)> as (_)" [100,55] 200) |
-  CaseVar lterm "string list" "nat list" "lterm list" ("Case/ (_)/ of/ <(_):=(_)>/ \<Rightarrow>/ (_)" [100,100,100,100]200) 
-    
-
-
-primrec shift_L :: "int \<Rightarrow> nat \<Rightarrow> lterm \<Rightarrow> lterm" where
-  "shift_L d c LTrue = LTrue" |
-  "shift_L d c LFalse = LFalse" |
-  "shift_L d c (LIf t1 t2 t3) = LIf (shift_L d c t1) (shift_L d c t2) (shift_L d c t3)" |
-  "shift_L d c (LVar k) = LVar (if k < c then k else nat (int k + d))" |
-  "shift_L d c (LNat n) = LNat n"|
-  "shift_L d c (LPlus t1 t2) = LPlus (shift_L d c t1) (shift_L d c t2)"|
-  "shift_L d c (LAbs T' t) = LAbs T' (shift_L d (Suc c) t)" |
-  "shift_L d c (LApp t1 t2) = LApp (shift_L d c t1) (shift_L d c t2)" |
-  "shift_L d c unit = unit" |
-  "shift_L d c (Seq t1 t2) = Seq (shift_L d c t1) (shift_L d c t2)" |
-  "shift_L d c (t as A) = (shift_L d c t) as A" |
-  "shift_L d c (Let var x := t in t1) = 
-    (if x\<ge> c then Let var (nat (int x + d)) := (shift_L d c t) in (shift_L d c t1)
-     else  Let var x := (shift_L d c t) in (shift_L d c t1)
-     )" |
-  "shift_L d c (\<lbrace>t1,t2\<rbrace>) = \<lbrace> shift_L d c t1 , shift_L d c t2 \<rbrace>" |
-  "shift_L d c (\<pi>1 t) = \<pi>1 (shift_L d c t)" |
-  "shift_L d c (\<pi>2 t) = \<pi>2 (shift_L d c t)" |
-  "shift_L d c (Tuple L) = Tuple (map (shift_L d c) L)" |
-  "shift_L d c (\<Pi> i t)   = \<Pi> i (shift_L d c t)" |
-  "shift_L d c (Record L LT)  = Record L (map (shift_L d c) LT)" |
-  "shift_L d c (ProjR l t) = ProjR l (shift_L d c t)" |
-  "shift_L d c (Pattern p) = <|p|>" |
-  "shift_L d c (Let pattern p := t1 in t2) = (Let pattern p := (shift_L d c t1) in (shift_L d c t2))" |
-  "shift_L d c (inl t as T') =  inl (shift_L d c t) as T'" |
-  "shift_L d c (inr t as T') =  inr (shift_L d c t) as T'" |
-  "shift_L d c (Case t of Inl x \<Rightarrow> t1 | Inr y \<Rightarrow> t2) = 
-    (Case (shift_L d c t) of 
-        Inl (if x\<ge> c then (nat (int x + d)) else x) \<Rightarrow> shift_L d c t1 
-      | Inr (if y\<ge> c then (nat (int y + d)) else y) \<Rightarrow> shift_L d c t2)" |
-  "shift_L d c (<l:=t> as A) = <l:= shift_L d c t> as A" |
-  "shift_L d c (Case t of <L:=I> \<Rightarrow> LT) = 
-    (Case (shift_L d c t) of <L:= (map (\<lambda>x. if x\<ge> c then (nat (int x + d)) else x) I)> \<Rightarrow> map (shift_L d c) LT)"
-
-function subst_L :: "nat \<Rightarrow> lterm \<Rightarrow> lterm \<Rightarrow> lterm" where
-  "subst_L j s LTrue = LTrue" |
-  "subst_L j s LFalse = LFalse" |
-  "subst_L j s (LIf t1 t2 t3) = LIf (subst_L j s t1) (subst_L j s t2) (subst_L j s t3)" |
-  "subst_L j s (LVar k) = (if k = j then s else LVar k)" |
-  "subst_L j s (LNat n) = LNat n"|
-  "subst_L j s (LPlus t1 t2) = LPlus (subst_L j s t1) (subst_L j s t2)"|
-  "subst_L j s (LAbs T' t) = LAbs T' (subst_L (Suc j) (shift_L 1 0 s) t)" |
-  "subst_L j s (LApp t1 t2) = LApp (subst_L j s t1) (subst_L j s t2)" |
-  "subst_L j s unit = unit" |
-  "subst_L j s (Seq t1 t2) = Seq (subst_L j s t1) (subst_L j s t2)" |
-  "subst_L j s (t as A) = (subst_L j s t) as A" |
-  "subst_L j s (Let var x := t in t1) = 
-  (if j=x then Let var x := subst_L j s t in t1
-    else  (Let var x := (subst_L j s t) in (subst_L j s t1))) " |
-  "subst_L j s (\<lbrace>t1,t2\<rbrace>) = \<lbrace>subst_L j s t1, subst_L j s t2\<rbrace>" |
-  "subst_L j s (\<pi>1 t) = \<pi>1 (subst_L j s t)" |
-  "subst_L j s (\<pi>2 t) = \<pi>2 (subst_L j s t)" |
-  "subst_L j s (\<Pi> i t) = \<Pi> i (subst_L j s t)" |
-  "subst_L j s (Tuple L) = Tuple (map (subst_L j s) L)" |
-  "subst_L j s (Record L LT) = Record L (map (subst_L j s) LT)" |
-  "subst_L j s (ProjR l t) = ProjR l (subst_L j s t)" |
-  "subst_L j s (Pattern p) = Pattern p" |
-  "subst_L j s (Let pattern p := t1 in t2) = (Let pattern p := (subst_L j s t1) in (subst_L j s t2))" |
-  "subst_L j s (inl t as T') =  inl (subst_L j s t) as T'" |
-  "subst_L j s (inr t as T') =  inr (subst_L j s t) as T'" |
-  "subst_L j s (Case t of Inl x \<Rightarrow> t1 | Inr y \<Rightarrow> t2) = 
-    (Case (subst_L j s t) of 
-        Inl x \<Rightarrow> (if j=x then t1 else subst_L j s t1)
-      | Inr y \<Rightarrow> (if j=y then t2 else subst_L j s t2))" |
-  "subst_L j s (<l:=t> as T') =  <l:=subst_L j s t> as T'" |
-  "subst_L j s (Case t of <L:=I> \<Rightarrow> LT) = 
-    (Case (subst_L j s t) of <L:=I> \<Rightarrow> map (\<lambda>p. if j=fst p then snd p else subst_L j s (snd p)) (zip I LT))"
-by pat_completeness auto
-
-termination
-  by (relation "measure (\<lambda>(j,s,t). size t)", auto)
-      (metis less_add_Suc1 size_list_estimation' set_zip_rightD lessI not_less)+
-  
-fun nbinder :: "lterm \<Rightarrow> nat" where
-"nbinder (LAbs A t) = Suc (nbinder t)" |
-"nbinder _ = 0" 
-
-text{*
-      We want to restrict the considered pattern matching and filling to coherent cases, which are
-      the cases when a pattern variable can only appear once in a given pattern.\\
-
-      Furthermore, the same coherence principle is valid for the pattern context. A pattern variable can only 
-      have on type at a time
-*}
-
-fun Pvars :: "Lpattern \<Rightarrow> nat list" where
-"Pvars (V n) = [n]" |
-"Pvars (RCD L PL) = (list_iter (\<lambda>x r. x @ r) [] (map Pvars PL))"
-
-
-fun patterns::"lterm \<Rightarrow> nat list" where
-"patterns (<|p|>) = Pvars p" |
-"patterns (LIf c t1 t2)               = patterns c @ patterns t1 @ patterns t2" |
-"patterns (LAbs A t1)                 = patterns t1" |
-"patterns (LApp t1 t2)                = patterns t1 @ patterns t2" |
-"patterns (Seq t1 t2)                 = patterns t1 @ patterns t2" |
-"patterns (t1 as A)                   = patterns t1" |
-"patterns (Let var x := t1 in t2)     = patterns t1 @ patterns t2" |
-"patterns (\<lbrace>t1,t2\<rbrace>)                   = patterns t1 @ patterns t2" |
-"patterns (Tuple L)                   = list_iter (\<lambda>e r. e @ r) [] (map (patterns) L)" |
-"patterns (Record L LT)               = list_iter (\<lambda>e r. e @ r) [] (map (patterns) LT)" |
-"patterns (\<pi>1 t)                      = patterns t" |
-"patterns (\<pi>2 t)                      = patterns t" |
-"patterns (\<Pi> i t)                     = patterns t" |
-"patterns (ProjR l t)                 = patterns t" |
-"patterns (Let pattern p := t1 in t2) = patterns t1 @ filter (\<lambda>x. x\<notin> set(Pvars p))(patterns t2)" |
-"patterns (inl t as T') =  patterns t" |
-"patterns (inr t as T') =  patterns t" |
-"patterns (Case t of Inl x \<Rightarrow> t1 | Inr y \<Rightarrow> t2) = patterns t @ patterns t1 @ patterns t2" |
-"patterns (<l:=t> as T') =  patterns t" |
-"patterns (Case t of <L:=I> \<Rightarrow> LT) = patterns t @ list_iter (\<lambda>e r. e @ r) [] (map (patterns) LT)" |
-"patterns t = []"
-
-inductive is_value_L :: "lterm \<Rightarrow> bool" where
-  VTrue : "is_value_L LTrue" |
-  VFalse: "is_value_L LFalse" |
-  VAbs  :"is_value_L (LAbs T' t)" |
-  VUnit :"is_value_L unit" |
-  VNat  : "is_value_L (LNat n)"|
-  VPair :"is_value_L v1 \<Longrightarrow> is_value_L v2 \<Longrightarrow> is_value_L (\<lbrace>v1,v2\<rbrace>)" |
-  VTuple:"(\<And>i.0\<le>i \<Longrightarrow> i<length L \<Longrightarrow> is_value_L (L!i)) \<Longrightarrow> is_value_L (Tuple L)" |
-  VRCD  :"(\<And>i.0\<le>i \<Longrightarrow> i<length LT \<Longrightarrow> is_value_L (LT!i)) \<Longrightarrow> is_value_L (Record L LT)"|
-  VSumL :"is_value_L v \<Longrightarrow> is_value_L (inl v as A)"|
-  VSumR :"is_value_L v \<Longrightarrow> is_value_L (inr v as A)"
-
-primrec FV :: "lterm \<Rightarrow> nat set" where
-  "FV LTrue = {}" |
-  "FV LFalse = {}" |
-  "FV (LIf t1 t2 t3) = FV t1 \<union> FV t2 \<union> FV t3" |
-  "FV (LVar x) = {x}" |
-  "FV (LNat n) = {}"|
-  "FV (LPlus t1 t2) = FV t1 \<union> FV t2"|
-  "FV (LAbs T1 t) = image (\<lambda>x. x - 1) (FV t - {0})" |
-  "FV (LApp t1 t2) = FV t1 \<union> FV t2" |
-  "FV unit = {}" |
-  "FV (Seq t1 t2) = FV t1 \<union> FV t2" |
-  "FV (t as A) = FV t" |
-  "FV (Let var x:= t in t1) = 
-    (if x \<in> FV t1 then (FV t1 - {x}) \<union> FV t else FV t1)" |
-  "FV (\<lbrace>t1,t2\<rbrace>) = FV t1 \<union> FV t2" |
-  "FV (\<pi>1 t) =  FV t" |
-  "FV (\<pi>2 t) =  FV t" |
-  "FV (Tuple L) = list_iter (\<lambda>x r. x \<union> r) {} (map FV L) "|
-  "FV (\<Pi> i t) = FV t" |
-  "FV (Record L LT) = list_iter (\<lambda>x r. x \<union> r) {} (map FV LT) "|
-  "FV (ProjR l t) = FV t" |
-  "FV (Pattern p) = {}" |
-  "FV (Let pattern p := t1 in t2) = FV t1 \<union> FV t2" |
-  "FV (inl t as A) = FV t" |
-  "FV (inr t as A) = FV t" |
-  "FV (Case t of Inl x \<Rightarrow> t1 | Inr y \<Rightarrow> t2) = FV t1 \<union> FV t2" |
-  "FV (<L:=t> as A) = FV t" |
-  "FV (Case t of <L:=I> \<Rightarrow> LT) = FV t \<union> list_iter (\<lambda>x r. x \<union> r) {} (map FV LT)" 
-
-
-text{*
-    We implement pattern matching and replacing with the following function and definition:
-    
-    \begin{itemize}
-      \item a \textbf{pattern context} 
-      \item a \textbf{pattern substitution} is a list of pairs (pattern var index, lterm)
-      \item \textbf{fill}, which will fill the patterns in a ltern with a lterm (based on a pattern substitution)
-      \item \textbf{Lmatch} is a predicate on a pattern, a value and a pattern substitution indicating 
-              if the pattern substitution associates the given pattern's variables to the corresponding part(s) of the
-              given value
-    \end{itemize}
-*}
-
-inductive same_dom:: "(nat \<Rightarrow> lterm) \<Rightarrow> nat list \<Rightarrow>bool" where
-  empty: "(\<And>x. f x = <|V x|>)\<Longrightarrow> same_dom f []" |
-  non_empty: "(\<And>x. x\<in>set A \<Longrightarrow> f x \<noteq> <|V x|>) \<Longrightarrow> same_dom f A"
-
-fun p_instantiate::"(nat\<Rightarrow> lterm) \<Rightarrow> Lpattern \<Rightarrow> lterm" where
-"p_instantiate \<Delta> (V k) = \<Delta> k"|
-"p_instantiate \<Delta> (RCD L PL) =  (if (same_dom \<Delta> (Pvars (RCD L PL)) \<and> (Pvars (RCD L PL)\<noteq>[])) then Record L (map (p_instantiate \<Delta>) PL)
-                                else <|RCD L PL|>)"
-
-fun fill::"(nat \<Rightarrow> lterm) \<Rightarrow> lterm \<Rightarrow> lterm" where
-"fill \<Delta> (Pattern p)                 = p_instantiate \<Delta> p" |
-"fill \<Delta> (LIf c t1 t2)               = LIf (fill \<Delta> c) (fill \<Delta> t1) (fill \<Delta> t2)" |
-"fill \<Delta> (LAbs A t1)                 = LAbs A (fill \<Delta> t1)" |
-"fill \<Delta> (LApp t1 t2)                = LApp (fill \<Delta> t1) (fill \<Delta> t2)" |
-"fill \<Delta> (LPlus t1 t2)                = LPlus (fill \<Delta> t1) (fill \<Delta> t2)" |
-"fill \<Delta> (Seq t1 t2)                 =  Seq (fill \<Delta> t1) (fill \<Delta> t2)" |
-"fill \<Delta> (t1 as A)                   = (fill \<Delta> t1) as A" |
-"fill \<Delta> (Let var x := t1 in t2)     = (Let var x := (fill \<Delta> t1) in (fill \<Delta> t2))" |
-"fill \<Delta> (\<lbrace>t1,t2\<rbrace>)                   = \<lbrace>(fill \<Delta> t1), (fill \<Delta> t2)\<rbrace>" |
-"fill \<Delta> (Tuple L)                   = Tuple (map (fill \<Delta>) L)" |
-"fill \<Delta> (Record L LT)               = Record L (map (fill \<Delta>) LT)" |
-"fill \<Delta> (\<pi>1 t)                      = \<pi>1 (fill \<Delta> t)" |
-"fill \<Delta> (\<pi>2 t)                      = \<pi>2 (fill \<Delta> t)" |
-"fill \<Delta> (\<Pi> i t)                     = \<Pi> i (fill \<Delta> t)" |
-"fill \<Delta> (ProjR l t)                 = ProjR l (fill \<Delta> t)" |
-"fill \<Delta> (Let pattern p := t1 in t2) = (Let pattern p := (fill \<Delta> t1) in (fill \<Delta> t2))" |
-"fill \<Delta> (inl t as A) = inl (fill \<Delta> t) as A"|
-"fill \<Delta> (inr t as A) = inr (fill \<Delta> t) as A"|
-"fill \<Delta> (Case t of Inl x \<Rightarrow> t1 | Inr y \<Rightarrow> t2) = (Case (fill \<Delta> t) of Inl x \<Rightarrow> (fill \<Delta> t1) | Inr y \<Rightarrow> (fill \<Delta> t2))"|
-"fill \<Delta> (<l:=t> as A) =  <l:=(fill \<Delta> t)> as A"|
-"fill \<Delta> (Case t of <L:=I> \<Rightarrow> LT) = (Case (fill \<Delta> t) of <L:=I> \<Rightarrow> map (fill \<Delta>) LT)"|
-"fill \<Delta> t = t"
 
 inductive Lmatch ::"Lpattern \<Rightarrow> lterm \<Rightarrow> (lterm \<Rightarrow>lterm) \<Rightarrow> bool" where
   M_Var:
@@ -292,7 +49,10 @@ inductive eval1_L :: "lterm \<Rightarrow> lterm \<Rightarrow> bool" where
   -- "Rules relating to the evaluation of Plus"
   eval1_LPlus:
     "eval1_L (LPlus (LNat n1) (LNat n2)) (LNat (n1+n2))"|
-
+  eval1_LUMinus:
+    "eval1_L (UMinus (LNat n1)) (LNat (-n1))" |
+  eval1_LIsZero:
+    "eval1_L (IsZero (LNat 0)) LTrue" |
  -- "Rules relating to evaluation of sequence"
   
   eval1_L_Seq:
@@ -388,10 +148,14 @@ inductive has_type_L :: "lcontext \<Rightarrow> lterm \<Rightarrow> pcontext \<R
   -- \<open>Rules relating to the type of the constructs of the $\lambda$-calculus\<close>
   has_type_LVar:
     "(x, T') |\<in>| \<Gamma> \<Longrightarrow> \<Gamma> \<turnstile> \<lparr>LVar x|;|fill \<delta>\<rparr> |:| (T')" |
-  have_type_LNat:
+  has_type_LNat:
     "\<Gamma> \<turnstile> \<lparr>LNat n|;| fill \<delta>\<rparr> |:| Nat"|
-  have_type_LPlus:
+  has_type_LPlus:
     "\<Gamma> \<turnstile> \<lparr>t1|;| fill \<delta>\<rparr> |:| Nat \<Longrightarrow> \<Gamma> \<turnstile> \<lparr>t2|;| fill \<delta>\<rparr> |:| Nat \<Longrightarrow> \<Gamma> \<turnstile> \<lparr>LPlus t1 t2|;| fill \<delta>\<rparr> |:| Nat" |  
+  has_type_UMinus:
+    "\<Gamma> \<turnstile> \<lparr>t|;| fill \<delta>\<rparr> |:| Nat \<Longrightarrow> \<Gamma> \<turnstile> \<lparr>UMinus t|;| fill \<delta>\<rparr> |:| Nat" |
+  has_type_IsZero:
+    "\<Gamma> \<turnstile> \<lparr>t|;| fill \<delta>\<rparr> |:| Nat \<Longrightarrow> \<Gamma> \<turnstile> \<lparr>IsZero t|;| fill \<delta>\<rparr> |:| Bool" |
   has_type_LAbs:
     "(\<Gamma> |,| T1) \<turnstile> \<lparr>t2|;| fill (shift_L 1 (Suc (nbinder t2)) \<circ> \<delta>)\<rparr> |:| T2 \<Longrightarrow> \<Gamma> \<turnstile> \<lparr>LAbs T1 t2|;|fill \<delta>\<rparr> |:| (T1 \<rightarrow> T2)" |
   has_type_LApp:
@@ -662,14 +426,14 @@ next
   case (has_type_ProjT i TL \<Gamma>1 t \<delta>1)
     show ?case
       using has_type_ProjT(4)[OF has_type_ProjT(5,6)]
-            "has_type_L.intros"(17)[OF has_type_ProjT(1,2)]
+            "has_type_L.intros"(19)[OF has_type_ProjT(1,2)]
       by fastforce
 next
   case (has_type_RCD L LT TL \<Gamma> \<delta>1)
     show ?case
       using has_type_RCD(1-4) nth_map[of _ LT "shift_L 1 n"]
             has_type_RCD(6)[OF _ has_type_RCD(7,8)]           
-      by (force intro!: "has_type_L.intros"(18))+
+      by (force intro!: "has_type_L.intros"(20))+
 next
   case (has_type_Let \<Gamma>1 t1 \<delta>1 A x t2 B)
     have 1:"n\<le>x \<Longrightarrow> ?case"
@@ -677,14 +441,14 @@ next
         assume le_x: "n\<le>x"
         show ?case
           using has_type_Let(4-6) le_x
-                "has_type_L.intros"(12)[OF has_type_Let(2)[OF has_type_Let(5,6)], of "Suc x"]
+                "has_type_L.intros"(14)[OF has_type_Let(2)[OF has_type_Let(5,6)], of "Suc x"]
           by  (simp add: le_x del: Fun.comp_apply,
                 metis insert_nth_take_drop rep_ins replace_inv_length append_Cons append_Nil2 append_eq_append_conv_if)
       qed
 
     have "n>x \<Longrightarrow> ?case"
       using has_type_Let(4-6) rep_ins2[OF _ has_type_Let(6), of x S A]
-            "has_type_L.intros"(12)[OF has_type_Let(2)[OF has_type_Let(5,6)], of x]
+            "has_type_L.intros"(14)[OF has_type_Let(2)[OF has_type_Let(5,6)], of x]
       by (simp del: Fun.comp_apply,
             metis append_Cons append_Nil insert_nth_take_drop replace_inv_length)
     with 1 show ?case 
@@ -697,8 +461,8 @@ next
         fix x
         show "(shift_L 1 n \<circ> (\<lambda>x. <|V x|>)) x = (\<lambda>x. <|V x|>) x" 
           using Fun.comp_apply[of "shift_L 1 n" "\<lambda>x. <|V x|>" x]
-                "shift_L.simps"(20)
-          by metis
+                "shift_L.simps"(22)
+          by (metis (full_types))
       qed
     have 1:"insert_nth n S \<Gamma>1 \<turnstile> \<lparr>(fill (shift_L 1 n \<circ> \<delta>) ^^ m) (<|V k|>)|;|id\<rparr> |:| A" 
       using has_type_PatternVar(2)[OF fill_id has_type_PatternVar(5)]
@@ -707,7 +471,7 @@ next
     have "set (patterns ((fill (shift_L 1 n \<circ> \<delta>) ^^ m) (<|V k|>))) = {}"
       using has_type_PatternVar(3,4) pattern_fill_shift[of m 1 n \<delta> "<|V k|>"]
       by fastforce  
-    with 1 show ?case by (auto intro:"has_type_L.intros"(20)[where \<delta>="(shift_L 1 n \<circ> \<delta>)"])
+    with 1 show ?case by (auto intro:"has_type_L.intros"(22)[where \<delta>="(shift_L 1 n \<circ> \<delta>)"])
 next
   case (has_type_LetPattern p t1 \<delta>1 \<Gamma>1 \<delta>2 B t2 A)
     have 1:"Lmatch p (shift_L 1 n t1) (shift_L 1 n \<circ> \<delta>1)"
@@ -762,7 +526,7 @@ next
              replace_inv_length not_le
       by metis+
     show ?case
-      by (auto)(insert A B1 B2 B3 B4 "has_type_L.intros"(25), force+)
+      by (auto)(insert A B1 B2 B3 B4 "has_type_L.intros"(27), force+)
 next
   case (has_type_CaseV L I TL LT \<Gamma> t \<delta>1 A)
     have branches_wtyped:"\<forall>i<length L.
@@ -815,7 +579,7 @@ next
     show ?case
       using has_type_CaseV(1-4) has_type_CaseV(6)[OF has_type_CaseV(8,9)]
             branches_wtyped
-      by (force intro!: "has_type_L.intros"(27))+      
+      by (force intro!: "has_type_L.intros"(29))+      
 qed (auto intro!: has_type_L.intros simp: nth_append min_def)
 
 lemma fill_keep_value:
@@ -830,6 +594,7 @@ lemma canonical_forms:
   "is_value_L v \<Longrightarrow> \<Gamma> \<turnstile> \<lparr>v|;|\<delta>\<rparr> |:| \<lparr>TL\<rparr> \<Longrightarrow> \<exists>L. is_value_L (Tuple L) \<and> v = Tuple L"
   "is_value_L v \<Longrightarrow> \<Gamma> \<turnstile> \<lparr>v|;|\<delta>\<rparr> |:| \<lparr>L|:|TL\<rparr> \<Longrightarrow> \<exists>L LT. is_value_L (Record L LT) \<and> v = (Record L LT)" 
   "is_value_L v \<Longrightarrow> \<Gamma> \<turnstile> \<lparr>v|;|\<delta>\<rparr> |:| A|+|B \<Longrightarrow> (\<exists>v1. is_value_L v1 \<and> v = inl v1 as A|+|B) \<or> (\<exists>v1. v = inr v1 as A|+|B \<and> is_value_L v1)" 
+  "is_value_L v \<Longrightarrow> \<Gamma> \<turnstile> \<lparr>v|;|\<delta>\<rparr> |:| Nat \<Longrightarrow> \<exists>n. v = LNat n"
 proof -
   assume  val: "is_value_L v" and 
           typed: "\<Gamma> \<turnstile> \<lparr>v|;|\<delta>\<rparr> |:| A|+|B"
