2016/Variant_Type_examples.thy
@@ -1,8 +1,11 @@
 theory Variant_Type_examples
 imports Main
         Ext_Structures
+        List
 begin
-  
+
+section{* Option Type *}
+
 abbreviation OptionType::"ltype \<Rightarrow> ltype" ("(_)/ option" [201]200) where
 "A option \<equiv> <[''none'',''some'']|,|[Unit,A]>"    
  
@@ -13,18 +16,86 @@ abbreviation emptyTable ::"lterm" where
 "emptyTable \<equiv> LAbs Nat (<''none'':=unit> as Nat option)"  
 
 
-lemma "\<emptyset> \<turnstile> \<lparr>emptyTable |;| id\<rparr> |:| Table"
+lemma emptyTable_well_typed:
+  "\<Gamma> \<turnstile> \<lparr>emptyTable |;| fill \<delta>\<rparr> |:| Table"
  proof -
+   
    let ?inner_term = "<''none'':= unit> as (Nat option)"
-   have H:"[Nat] \<turnstile> \<lparr> ?inner_term|;| fill (shift_L 1 (Suc (nbinder ?inner_term))\<circ>(\<lambda>x. <|V x|>))\<rparr> |:| Nat option"
-     using has_type_Variant[of "[Nat]" unit "shift_L 1 (Suc (nbinder ?inner_term))\<circ>(\<lambda>x. <|V x|>)" "[Unit, Nat]" 0 "[''none'',''some'']"]
-           has_type_LUnit[of "[Nat]" "shift_L 1 (Suc (nbinder ?inner_term))\<circ>(\<lambda>x. <|V x|>)"] fill_id
+   have H:" \<Gamma> |,| Nat \<turnstile> \<lparr> ?inner_term|;| fill (shift_L 1 (Suc (nbinder ?inner_term))\<circ>\<delta>)\<rparr> |:| Nat option"
+     using has_type_Variant[of "\<Gamma>|,|Nat" unit "shift_L 1 (Suc (nbinder ?inner_term))\<circ>\<delta>" "[Unit, Nat]" 0 "[''none'',''some'']"]
+           has_type_LUnit[of "\<Gamma>|,|Nat" "shift_L 1 (Suc (nbinder ?inner_term))\<circ>\<delta>"] fill_id
      by fastforce
    
    then show ?thesis     
-     using has_type_LAbs[of Nat \<emptyset> ?inner_term "\<lambda>x. <|V x|>" "Nat option"]
+     using has_type_LAbs[of Nat "\<Gamma>" ?inner_term \<delta> "Nat option"]
            fill_id     
      by auto
 qed
-      
+   
+abbreviation Lequal :: "lterm\<Rightarrow>lterm\<Rightarrow>lterm" where
+"Lequal n m\<equiv> LApp (LApp (LAbs Nat (LAbs Nat (IsZero (LPlus (UMinus (LVar 0)) (LVar 1))))) n) m"
+
+abbreviation extendTable :: "lterm" where
+"extendTable \<equiv> LAbs Table (LAbs Nat (LAbs Nat (LAbs Nat 
+                  (LIf (Lequal (LVar 0) (LVar 2)) (<''some'':= LVar 1> as Nat option) (LApp (LVar 3) (LVar 0))
+                          ))))"
+
+lemma Lequal_well_typed:
+ "\<Gamma>\<turnstile> \<lparr>n |;| fill \<delta>\<rparr> |:| Nat \<Longrightarrow> \<Gamma> \<turnstile> \<lparr>m |;| fill \<delta>\<rparr> |:| Nat \<Longrightarrow> \<Gamma> \<turnstile> \<lparr>Lequal n m |;| fill \<delta> \<rparr> |:| Bool" 
+proof -
+  assume args_types:"\<Gamma>\<turnstile> \<lparr>n |;| fill \<delta>\<rparr> |:| Nat" "\<Gamma> \<turnstile> \<lparr>m |;| fill \<delta>\<rparr> |:| Nat"
+  
+  have V1:" (Suc 0, Nat) |\<in>| (\<Gamma> |,| ltype.Nat |,| ltype.Nat)" by auto
+  have V0:" (0, Nat) |\<in>| (\<Gamma> |,| ltype.Nat |,| ltype.Nat)" by auto
+
+  have "\<Gamma> |,| ltype.Nat |,| ltype.Nat  \<turnstile> 
+        \<lparr>IsZero (LPlus (UMinus (LVar 0)) (LVar (Suc 0)))|;|fill (shift_L 1 (Suc 0) \<circ> (shift_L 1 (Suc (Suc 0)) \<circ> \<delta>))\<rparr> |:| Bool" 
+   using has_type_LPlus  has_type_UMinus has_type_IsZero
+         has_type_LVar[OF V0,of "shift_L 1 (Suc 0) \<circ> (shift_L 1 (Suc (Suc 0)) \<circ> \<delta>)"]
+         has_type_LVar[OF V1,of "shift_L 1 (Suc 0) \<circ> (shift_L 1 (Suc (Suc 0)) \<circ> \<delta>)"]         
+   by blast
+  then show "\<Gamma> \<turnstile> \<lparr>Lequal n m |;| fill \<delta> \<rparr> |:| Bool"
+    using has_type_LApp[OF has_type_LApp[OF _ args_types(1)] args_types(2)]
+          has_type_LAbs
+    by auto
+qed   
+
+lemma shift_cumul[simp]:
+  "(shift_L d c \<circ> shift_L d c) = shift_L (d+d) c"
+sorry
+
+lemma extendTable_well_typed:
+  "\<Gamma>\<turnstile> \<lparr> extendTable |;| fill \<delta>\<rparr> |:| Table\<rightarrow>Nat\<rightarrow>Nat\<rightarrow>Table"
+proof-
+  let ?ctx = "\<Gamma> |,| Table |,| ltype.Nat |,| ltype.Nat |,| ltype.Nat" and
+      ?delta = "shift_L 1 (Suc 0) \<circ>
+                         (shift_L 1 (Suc (Suc 0)) \<circ> (shift_L 1 (Suc (Suc (Suc 0))) \<circ> (shift_L 1 (Suc (Suc (Suc (Suc 0)))) \<circ> \<delta>)))"
+  
+  have 1: "?ctx \<turnstile> \<lparr>Lequal (LVar 0) (LVar 2)|;|fill ?delta \<rparr> |:| Bool" 
+    using Lequal_well_typed[of ?ctx _ ?delta]
+          has_type_LVar[of _ Nat ?ctx ?delta]
+    by fastforce
+
+  have 2: "?ctx \<turnstile> \<lparr><''some'':= LVar 1> as Nat option |;|fill ?delta \<rparr> |:| Nat option" 
+    using has_type_Variant[of ?ctx "LVar 1" ?delta "[Unit,Nat]" 1 "[''none'',''some'']"]
+          has_type_LVar[of _ Nat ?ctx ?delta]
+    by force
+
+  have "?ctx \<turnstile> \<lparr>LApp (LVar 3) (LVar 0) |;|fill ?delta \<rparr> |:| Nat option"
+    using has_type_LApp[of ?ctx "LVar 3" ?delta Nat "Nat option" "LVar 0"] 
+          has_type_LVar[of _ _ ?ctx ?delta]
+    by auto
+
+  with 1 2 show ?thesis 
+    using has_type_LAbs has_type_LIf[of ?ctx "Lequal (LVar 0) (LVar 2)" ?delta]
+    by force
+qed
+
+section{* Enumerations*}
+
+abbreviation Weekday :: "ltype" where
+  "Weekday \<equiv> <[''monday'',''tuesday'',''wednesday'',''thursday'',''friday'']|,|(replicate 5 Unit)>"
+
+
+
 end
