2016/Lambda_calculus.thy
@@ -1,0 +1,273 @@
+theory Lambda_calculus
+imports Main
+        List_extra
+        "$AFP/List-Index/List_Index"
+begin
+
+  datatype ltype =
+  Nat  |
+  Bool |
+  T (num:nat) |
+  Unit |
+  Prod ltype ltype (infix "|\<times>|" 225)|
+  Fun (domain: ltype) (codomain: ltype) (infixr "\<rightarrow>" 225)|
+  TupleT "ltype list" ( "\<lparr>_\<rparr>" [150]225) |
+  RecordT "string list" "ltype list" ( "\<lparr>_|:|_\<rparr>" [150,150] 225) |
+  Sum ltype ltype (infix "|+|" 225) |
+  TVariant "string list" "ltype list" ( "<_|,|_>" [150,150] 225) 
+  
+datatype Lpattern = V nat | RCD "string list" "Lpattern list"
+
+datatype lterm =
+  LTrue |
+  LFalse |
+  LIf (bool_expr: lterm) (then_expr: lterm) (else_expr: lterm) |
+  LVar nat |
+  LNat int |
+  LPlus lterm lterm |
+  UMinus lterm |
+  IsZero lterm |
+  LAbs (arg_type: ltype) (body: lterm) |
+  LApp lterm lterm |
+  unit |
+  Seq (fp: lterm) (sp: lterm) ("(_;;_)" [100,50] 200) |
+  AS lterm ltype ("_/ as/ _" [100,150] 200) |
+  LetBinder nat lterm lterm ("Let/ var/ (_)/ :=/ (_)/ in/ (_)" [100,120,150] 250) | 
+  Pair lterm lterm ("\<lbrace>_,_\<rbrace>" [100,150] 250) |
+  Proj1 lterm ("\<pi>1/ _" [100] 250) |
+  Proj2 lterm ("\<pi>2/ _" [100] 250) |
+  Tuple "lterm list" |
+  ProjT nat lterm ("\<Pi>/ _/ (_)" [100,150] 250) |
+  Record "string list" "lterm list" |
+  ProjR string lterm |
+  Pattern Lpattern ("<|_|>" [100] 250) |
+  LetP Lpattern lterm lterm ("Let/ pattern/ (_)/ :=/ (_)/ in/ (_)"[100,120,150]250) |
+  inl lterm ltype ("inl/ (_)/ as/ (_)" [100,100]200) |
+  inr lterm ltype ("inr/ (_)/ as/ (_)" [100,100]200) |
+  CaseSum lterm nat lterm nat lterm ("Case/ (_)/ of/ Inl/ (_)/ \<Rightarrow>/ (_)/ |/ Inr/ (_)/ \<Rightarrow>/ (_)" [100, 100,100, 100, 100]200) |
+  Variant string lterm ltype ("<(_):=(_)> as (_)" [100,55] 200) |
+  CaseVar lterm "string list" "nat list" "lterm list" ("Case/ (_)/ of/ <(_):=(_)>/ \<Rightarrow>/ (_)" [100,100,100,100]200)|
+  Fixpoint "lterm"  ("fix (_)" [201]200)
+    
+
+primrec shift_L :: "int \<Rightarrow> nat \<Rightarrow> lterm \<Rightarrow> lterm" where
+  "shift_L d c LTrue = LTrue" |
+  "shift_L d c LFalse = LFalse" |
+  "shift_L d c (LIf t1 t2 t3) = LIf (shift_L d c t1) (shift_L d c t2) (shift_L d c t3)" |
+  "shift_L d c (LVar k) = LVar (if k < c then k else nat (int k + d))" |
+  "shift_L d c (LNat n) = LNat n"|
+  "shift_L d c (UMinus t) = UMinus (shift_L d c t)"|
+  "shift_L d c (IsZero t) = IsZero (shift_L d c t)"|
+  "shift_L d c (LPlus t1 t2) = LPlus (shift_L d c t1) (shift_L d c t2)"|
+  "shift_L d c (LAbs T' t) = LAbs T' (shift_L d (Suc c) t)" |
+  "shift_L d c (LApp t1 t2) = LApp (shift_L d c t1) (shift_L d c t2)" |
+  "shift_L d c unit = unit" |
+  "shift_L d c (Seq t1 t2) = Seq (shift_L d c t1) (shift_L d c t2)" |
+  "shift_L d c (t as A) = (shift_L d c t) as A" |
+  "shift_L d c (Let var x := t in t1) = 
+    (if x\<ge> c then Let var (nat (int x + d)) := (shift_L d c t) in (shift_L d c t1)
+     else  Let var x := (shift_L d c t) in (shift_L d c t1)
+     )" |
+  "shift_L d c (\<lbrace>t1,t2\<rbrace>) = \<lbrace> shift_L d c t1 , shift_L d c t2 \<rbrace>" |
+  "shift_L d c (\<pi>1 t) = \<pi>1 (shift_L d c t)" |
+  "shift_L d c (\<pi>2 t) = \<pi>2 (shift_L d c t)" |
+  "shift_L d c (Tuple L) = Tuple (map (shift_L d c) L)" |
+  "shift_L d c (\<Pi> i t)   = \<Pi> i (shift_L d c t)" |
+  "shift_L d c (Record L LT)  = Record L (map (shift_L d c) LT)" |
+  "shift_L d c (ProjR l t) = ProjR l (shift_L d c t)" |
+  "shift_L d c (Pattern p) = <|p|>" |
+  "shift_L d c (Let pattern p := t1 in t2) = (Let pattern p := (shift_L d c t1) in (shift_L d c t2))" |
+  "shift_L d c (inl t as T') =  inl (shift_L d c t) as T'" |
+  "shift_L d c (inr t as T') =  inr (shift_L d c t) as T'" |
+  "shift_L d c (Case t of Inl x \<Rightarrow> t1 | Inr y \<Rightarrow> t2) = 
+    (Case (shift_L d c t) of 
+        Inl (if x\<ge> c then (nat (int x + d)) else x) \<Rightarrow> shift_L d c t1 
+      | Inr (if y\<ge> c then (nat (int y + d)) else y) \<Rightarrow> shift_L d c t2)" |
+  "shift_L d c (<l:=t> as A) = <l:= shift_L d c t> as A" |
+  "shift_L d c (Case t of <L:=I> \<Rightarrow> LT) = 
+    (Case (shift_L d c t) of <L:= (map (\<lambda>x. if x\<ge> c then (nat (int x + d)) else x) I)> \<Rightarrow> map (shift_L d c) LT)"|
+  "shift_L d c (Fixpoint t) = Fixpoint (shift_L d c t)"
+
+
+function subst_L :: "nat \<Rightarrow> lterm \<Rightarrow> lterm \<Rightarrow> lterm" where
+  "subst_L j s LTrue = LTrue" |
+  "subst_L j s LFalse = LFalse" |
+  "subst_L j s (LIf t1 t2 t3) = LIf (subst_L j s t1) (subst_L j s t2) (subst_L j s t3)" |
+  "subst_L j s (LVar k) = (if k = j then s else LVar k)" |
+  "subst_L j s (LNat n) = LNat n"|
+  "subst_L j s (UMinus t) = UMinus (subst_L j s t)"|
+  "subst_L j s (IsZero t) = IsZero (subst_L j s t)"|
+  "subst_L j s (LPlus t1 t2) = LPlus (subst_L j s t1) (subst_L j s t2)"|
+  "subst_L j s (LAbs T' t) = LAbs T' (subst_L (Suc j) (shift_L 1 0 s) t)" |
+  "subst_L j s (LApp t1 t2) = LApp (subst_L j s t1) (subst_L j s t2)" |
+  "subst_L j s unit = unit" |
+  "subst_L j s (Seq t1 t2) = Seq (subst_L j s t1) (subst_L j s t2)" |
+  "subst_L j s (t as A) = (subst_L j s t) as A" |
+  "subst_L j s (Let var x := t in t1) = 
+  (if j=x then Let var x := subst_L j s t in t1
+    else  (Let var x := (subst_L j s t) in (subst_L j s t1))) " |
+  "subst_L j s (\<lbrace>t1,t2\<rbrace>) = \<lbrace>subst_L j s t1, subst_L j s t2\<rbrace>" |
+  "subst_L j s (\<pi>1 t) = \<pi>1 (subst_L j s t)" |
+  "subst_L j s (\<pi>2 t) = \<pi>2 (subst_L j s t)" |
+  "subst_L j s (\<Pi> i t) = \<Pi> i (subst_L j s t)" |
+  "subst_L j s (Tuple L) = Tuple (map (subst_L j s) L)" |
+  "subst_L j s (Record L LT) = Record L (map (subst_L j s) LT)" |
+  "subst_L j s (ProjR l t) = ProjR l (subst_L j s t)" |
+  "subst_L j s (Pattern p) = Pattern p" |
+  "subst_L j s (Let pattern p := t1 in t2) = (Let pattern p := (subst_L j s t1) in (subst_L j s t2))" |
+  "subst_L j s (inl t as T') =  inl (subst_L j s t) as T'" |
+  "subst_L j s (inr t as T') =  inr (subst_L j s t) as T'" |
+  "subst_L j s (Case t of Inl x \<Rightarrow> t1 | Inr y \<Rightarrow> t2) = 
+    (Case (subst_L j s t) of 
+        Inl x \<Rightarrow> (if j=x then t1 else subst_L j s t1)
+      | Inr y \<Rightarrow> (if j=y then t2 else subst_L j s t2))" |
+  "subst_L j s (<l:=t> as T') =  <l:=subst_L j s t> as T'" |
+  "subst_L j s (Case t of <L:=I> \<Rightarrow> LT) = 
+    (Case (subst_L j s t) of <L:=I> \<Rightarrow> map (\<lambda>p. if j=fst p then snd p else subst_L j s (snd p)) (zip I LT))" |
+  "subst_L j s (Fixpoint t) = Fixpoint (subst_L j s t)"
+by pat_completeness auto
+
+termination
+  by (relation "measure (\<lambda>(j,s,t). size t)", auto)
+      (metis less_add_Suc1 size_list_estimation' set_zip_rightD lessI not_less)+
+  
+fun nbinder :: "lterm \<Rightarrow> nat" where
+"nbinder (LAbs A t) = Suc (nbinder t)" |
+"nbinder _ = 0" 
+
+text{*
+      We want to restrict the considered pattern matching and filling to coherent cases, which are
+      the cases when a pattern variable can only appear once in a given pattern.\\
+
+      Furthermore, the same coherence principle is valid for the pattern context. A pattern variable can only 
+      have on type at a time
+*}
+
+fun Pvars :: "Lpattern \<Rightarrow> nat list" where
+"Pvars (V n) = [n]" |
+"Pvars (RCD L PL) = (list_iter (\<lambda>x r. x @ r) [] (map Pvars PL))"
+
+
+fun patterns::"lterm \<Rightarrow> nat list" where
+"patterns (<|p|>) = Pvars p" |
+"patterns (LIf c t1 t2)               = patterns c @ patterns t1 @ patterns t2" |
+"patterns (LPlus t1 t2)               = patterns t1 @ patterns t2" |
+"patterns (UMinus t)                  = patterns t" |
+"patterns (IsZero t)                  = patterns t" |
+"patterns (LAbs A t1)                 = patterns t1" |
+"patterns (LApp t1 t2)                = patterns t1 @ patterns t2" |
+"patterns (Seq t1 t2)                 = patterns t1 @ patterns t2" |
+"patterns (t1 as A)                   = patterns t1" |
+"patterns (Let var x := t1 in t2)     = patterns t1 @ patterns t2" |
+"patterns (\<lbrace>t1,t2\<rbrace>)                   = patterns t1 @ patterns t2" |
+"patterns (Tuple L)                   = list_iter (\<lambda>e r. e @ r) [] (map (patterns) L)" |
+"patterns (Record L LT)               = list_iter (\<lambda>e r. e @ r) [] (map (patterns) LT)" |
+"patterns (\<pi>1 t)                      = patterns t" |
+"patterns (\<pi>2 t)                      = patterns t" |
+"patterns (\<Pi> i t)                     = patterns t" |
+"patterns (ProjR l t)                 = patterns t" |
+"patterns (Let pattern p := t1 in t2) = patterns t1 @ filter (\<lambda>x. x\<notin> set(Pvars p))(patterns t2)" |
+"patterns (inl t as T') =  patterns t" |
+"patterns (inr t as T') =  patterns t" |
+"patterns (Case t of Inl x \<Rightarrow> t1 | Inr y \<Rightarrow> t2) = patterns t @ patterns t1 @ patterns t2" |
+"patterns (<l:=t> as T') =  patterns t" |
+"patterns (Case t of <L:=I> \<Rightarrow> LT) = patterns t @ list_iter (\<lambda>e r. e @ r) [] (map (patterns) LT)" |
+"patterns (Fixpoint t) = patterns t"|
+"patterns t = []"
+
+
+inductive is_value_L :: "lterm \<Rightarrow> bool" where
+  VTrue : "is_value_L LTrue" |
+  VFalse: "is_value_L LFalse" |
+  VAbs  :"is_value_L (LAbs T' t)" |
+  VUnit :"is_value_L unit" |
+  VNat  : "is_value_L (LNat n)"|
+  VPair :"is_value_L v1 \<Longrightarrow> is_value_L v2 \<Longrightarrow> is_value_L (\<lbrace>v1,v2\<rbrace>)" |
+  VTuple:"(\<And>i.0\<le>i \<Longrightarrow> i<length L \<Longrightarrow> is_value_L (L!i)) \<Longrightarrow> is_value_L (Tuple L)" |
+  VRCD  :"(\<And>i.0\<le>i \<Longrightarrow> i<length LT \<Longrightarrow> is_value_L (LT!i)) \<Longrightarrow> is_value_L (Record L LT)"|
+  VSumL :"is_value_L v \<Longrightarrow> is_value_L (inl v as A)"|
+  VSumR :"is_value_L v \<Longrightarrow> is_value_L (inr v as A)"
+
+primrec FV :: "lterm \<Rightarrow> nat set" where
+  "FV LTrue = {}" |
+  "FV LFalse = {}" |
+  "FV (LIf t1 t2 t3) = FV t1 \<union> FV t2 \<union> FV t3" |
+  "FV (LVar x) = {x}" |
+  "FV (LNat n) = {}"|
+  "FV (LPlus t1 t2) = FV t1 \<union> FV t2"|
+  "FV (UMinus t) = FV t"|
+  "FV (IsZero t) = FV t"|
+  "FV (LAbs T1 t) = image (\<lambda>x. x - 1) (FV t - {0})" |
+  "FV (LApp t1 t2) = FV t1 \<union> FV t2" |
+  "FV unit = {}" |
+  "FV (Seq t1 t2) = FV t1 \<union> FV t2" |
+  "FV (t as A) = FV t" |
+  "FV (Let var x:= t in t1) = 
+    (if x \<in> FV t1 then (FV t1 - {x}) \<union> FV t else FV t1)" |
+  "FV (\<lbrace>t1,t2\<rbrace>) = FV t1 \<union> FV t2" |
+  "FV (\<pi>1 t) =  FV t" |
+  "FV (\<pi>2 t) =  FV t" |
+  "FV (Tuple L) = list_iter (\<lambda>x r. x \<union> r) {} (map FV L) "|
+  "FV (\<Pi> i t) = FV t" |
+  "FV (Record L LT) = list_iter (\<lambda>x r. x \<union> r) {} (map FV LT) "|
+  "FV (ProjR l t) = FV t" |
+  "FV (Pattern p) = {}" |
+  "FV (Let pattern p := t1 in t2) = FV t1 \<union> FV t2" |
+  "FV (inl t as A) = FV t" |
+  "FV (inr t as A) = FV t" |
+  "FV (Case t of Inl x \<Rightarrow> t1 | Inr y \<Rightarrow> t2) = FV t1 \<union> FV t2" |
+  "FV (<L:=t> as A) = FV t" |
+  "FV (Case t of <L:=I> \<Rightarrow> LT) = FV t \<union> list_iter (\<lambda>x r. x \<union> r) {} (map FV LT)" |
+  "FV (Fixpoint t) = FV t"
+
+
+text{*
+    We implement pattern matching and replacing with the following function and definition:
+    
+    \begin{itemize}
+      \item a \textbf{pattern context} 
+      \item a \textbf{pattern substitution} is a list of pairs (pattern var index, lterm)
+      \item \textbf{fill}, which will fill the patterns in a ltern with a lterm (based on a pattern substitution)
+      \item \textbf{Lmatch} is a predicate on a pattern, a value and a pattern substitution indicating 
+              if the pattern substitution associates the given pattern's variables to the corresponding part(s) of the
+              given value
+    \end{itemize}
+*}
+
+inductive same_dom:: "(nat \<Rightarrow> lterm) \<Rightarrow> nat list \<Rightarrow>bool" where
+  empty: "(\<And>x. f x = <|V x|>)\<Longrightarrow> same_dom f []" |
+  non_empty: "(\<And>x. x\<in>set A \<Longrightarrow> f x \<noteq> <|V x|>) \<Longrightarrow> same_dom f A"
+
+fun p_instantiate::"(nat\<Rightarrow> lterm) \<Rightarrow> Lpattern \<Rightarrow> lterm" where
+"p_instantiate \<Delta> (V k) = \<Delta> k"|
+"p_instantiate \<Delta> (RCD L PL) =  (if (same_dom \<Delta> (Pvars (RCD L PL)) \<and> (Pvars (RCD L PL)\<noteq>[])) then Record L (map (p_instantiate \<Delta>) PL)
+                                else <|RCD L PL|>)"
+
+fun fill::"(nat \<Rightarrow> lterm) \<Rightarrow> lterm \<Rightarrow> lterm" where
+"fill \<Delta> (Pattern p)                 = p_instantiate \<Delta> p" |
+"fill \<Delta> (LIf c t1 t2)               = LIf (fill \<Delta> c) (fill \<Delta> t1) (fill \<Delta> t2)" |
+"fill \<Delta> (LAbs A t1)                 = LAbs A (fill \<Delta> t1)" |
+"fill \<Delta> (LApp t1 t2)                = LApp (fill \<Delta> t1) (fill \<Delta> t2)" |
+"fill \<Delta> (LPlus t1 t2)               = LPlus (fill \<Delta> t1) (fill \<Delta> t2)" |
+"fill \<Delta> (UMinus t)                  = UMinus (fill \<Delta> t)" |
+"fill \<Delta> (IsZero t)                  = IsZero (fill \<Delta> t)" |
+"fill \<Delta> (Seq t1 t2)                 =  Seq (fill \<Delta> t1) (fill \<Delta> t2)" |
+"fill \<Delta> (t1 as A)                   = (fill \<Delta> t1) as A" |
+"fill \<Delta> (Let var x := t1 in t2)     = (Let var x := (fill \<Delta> t1) in (fill \<Delta> t2))" |
+"fill \<Delta> (\<lbrace>t1,t2\<rbrace>)                   = \<lbrace>(fill \<Delta> t1), (fill \<Delta> t2)\<rbrace>" |
+"fill \<Delta> (Tuple L)                   = Tuple (map (fill \<Delta>) L)" |
+"fill \<Delta> (Record L LT)               = Record L (map (fill \<Delta>) LT)" |
+"fill \<Delta> (\<pi>1 t)                      = \<pi>1 (fill \<Delta> t)" |
+"fill \<Delta> (\<pi>2 t)                      = \<pi>2 (fill \<Delta> t)" |
+"fill \<Delta> (\<Pi> i t)                     = \<Pi> i (fill \<Delta> t)" |
+"fill \<Delta> (ProjR l t)                 = ProjR l (fill \<Delta> t)" |
+"fill \<Delta> (Let pattern p := t1 in t2) = (Let pattern p := (fill \<Delta> t1) in (fill \<Delta> t2))" |
+"fill \<Delta> (inl t as A) = inl (fill \<Delta> t) as A"|
+"fill \<Delta> (inr t as A) = inr (fill \<Delta> t) as A"|
+"fill \<Delta> (Case t of Inl x \<Rightarrow> t1 | Inr y \<Rightarrow> t2) = (Case (fill \<Delta> t) of Inl x \<Rightarrow> (fill \<Delta> t1) | Inr y \<Rightarrow> (fill \<Delta> t2))"|
+"fill \<Delta> (<l:=t> as A) =  <l:=(fill \<Delta> t)> as A"|
+"fill \<Delta> (Case t of <L:=I> \<Rightarrow> LT) = (Case (fill \<Delta> t) of <L:=I> \<Rightarrow> map (fill \<Delta>) LT)"|
+"fill \<Delta> (Fixpoint t) = Fixpoint (fill \<Delta> t)" |
+"fill \<Delta> t = t"
+
+end
